test_proof.lean
@@ -1,0 +1,6 @@
+import Project.FactorizationForest.Forest
+
+open FactorizationForest
+
+  induction u, hu, s using buildFactorizationTree.induct eval with
+  | case1 => sorry
